coq/proof/SimulationLocal.v
@@ -126,7 +126,7 @@ Section SimLocal.
       (STEP:
          forall st3_tgt event
            (STEP: sInsn conf_tgt st1_tgt st3_tgt event),
-         exists st2_src st3_src st3_tgt inv3 idx3,
+         exists st2_src st3_src inv3 idx3,
            <<TAU: sop_star conf_src st1_src st2_src E0>> /\
            <<EVT: sInsn_indexed conf_src st2_src st3_src idx1 idx3 event>> /\
            <<MEMLE: InvMem.Rel.le inv1 inv3>> /\
