coq/proof/SoundPostcondCall.v
@@ -90,10 +90,6 @@ Lemma postcond_call_sound
                    st0_tgt.(ECS) mem1_tgt)
           invst1 invmem1 inv1>>>>.
 Proof.
-  (* TODO: proof crashed since we remove postcond_cmd_forget *)
-  (* unfold Postcond.postcond_cmd, Postcond.postcond_cmd_forget in *. *)
-  (* splits; ss. *)
-  (* - admit. (* fun *) *)
-  (* - admit. (* args *) *)
-  (* - admit. (* return *) *)
+  unfold Postcond.postcond_cmd in *.
+  admit.
 Admitted.
